\documentclass{article}
\usepackage{mathpartir}
\usepackage{amsmath}
\usepackage{mttex/mttex}
\usepackage{bm}

\newcommand{\sfontnonterm}[1]{\sfont{\emph{#1}}}
\newlanguage{\scolor}{\sfontnonterm}{\sfontsym}{s}
{x,e,v,E}
{}
{}
{}

\newcommand{\sfune}[2]{(\sfontsym{\lambda}#1.#2)}
\newcommand{\sappe}[2]{(#1\; #2)}
\newcommand{\ssetbange}[2]{(\sfont{set!}\; #1\; #2)}
\newcommand{\slete}[2]{(\sfont{let}\; (#1)\; #2)}
\newcommand{\sbegine}[2]{(\sfont{begin}\; #1\; #2)}
\newcommand{\SAe}[1]{\sfont{S}\tfont{A}(#1)}

\newcommand{\tfontnonterm}[1]{\emph{\tcolor{$\bm{#1}$}}}
\newlanguage{\tcolor}{\tfontnonterm}{\tfontsym}{t}
{x,M,V,N,E}
{}
{}
{}


\newcommand{\tfune}[2]{\tfontsym{\lambda}#1. #2}

\begin{document}

$$
\begin{array}{rcl}
  \se & ::= & \sx \mid \sfune{\sx}{\se} \mid \sappe{\se}{\se} \mid \ssetbange{\sx}{\se} \mid \slete{[\sx\; \se]\; \dots}{\se} \mid \sbegine{\se}{\dots} \mid .... \\&&
  \mid \SAe{\tM}
\end{array}
$$


$$
\begin{array}{rcl}
V & ::= & x \mid (\lambda x.M) \mid \textrm{true} \mid \textrm{false} \mid .... \\ && AS(e) \\
N & ::= & V \mid (V\; V) \mid (\textrm{set!}\; x\; V) \mid .... \\ && AS(e) \\
M & ::= & N \mid (\textrm{let}\; ([x\; N]\; ...)\; M) \mid (\textrm{begin}\; N\; ...\; M) \mid (\textrm{if}\; V\; M\; M) \mid .... \\ && AS(e) \\
\end{array}
$$

$$
\begin{array}{rcl}
  v & ::= & (\lambda x.e) \mid true \mid .... \\
  E & ::= & [\cdot] \mid E\; e \mid v\; E \mid .... \\
  H & ::= & \cdot \mid H,x \mapsto v
\end{array}
$$

\fbox{$H;\; e \to H;\; e$}
\begin{mathpar}
\begin{array}{rcl}
  (\lambda x.e)\; v & \to & e[x\; := v] \\
  & \vdots

\end{array}

\inferrule
{e \to e'}
{E[e] \to E[e']}
\end{mathpar}


$$
\begin{array}{rcl}
  E & ::= & [\cdot] \mid (\textrm{let} ([x\; V]\; ... [x\; [\cdot]] [x\; N]\; ...)\; M) \\
  H & ::= & \cdot \mid H,x \mapsto V
\end{array}
$$


\fbox{$H;\; M \to H;\; M$}
\begin{mathpar}
\begin{array}{rclr}
  (\lambda x.M)\; V & \to & M[x\; := V] \\
  &\vdots& \\
  (\textrm{let}\; ([x\; V]\; ...)\; M) & \to & M[x := V\; ...]
\end{array}
\end{mathpar}

\fbox{$e \to^a e$}
\begin{mathpar}
  \begin{array}{rclr}
    M & \to^a & SA(M) & \textrm{[A-normal]} \\[2pt]

    E[(\textrm{let}\; ([x\; e]\; ...)\; e_2] & \to^a &
    SA(\textrm{let}\; ([x\; AS(e)]\; ...)\; AS(E[e_2])) & \textrm{[A-merge-let]} \\[2pt]

    E[(\textrm{begin}\; e_1\; ...\; e_2)] & \to^a &
    SA(\textrm{begin}\; AS(e_1)\; ...\; AS(E[e_2])) & \textrm{[A-merge-begin]} \\[2pt]

    E[N] & \to^a & SA(\textrm{let}\; ([x\; N])\; AS(E[x])) & \textrm{[A-lift]} \\
    && \text{where $E$ is not an ``$N$ accepting target context''} \\
    && \text{and $N$ is not a $V$} \\
    & \vdots &
  \end{array}
\end{mathpar}

\begin{mathpar}
  \begin{array}{rcl}
    p & ::= & e \mid M \\
    T & ::= & AS(C_M) \\
    C_M & ::= & [\cdot] \mid
     (\textrm{let}\; ([x\; N]\; ...) C_M) \mid ....
  \end{array}
\end{mathpar}

\fbox{$M\; {}^s\!\!\to^a M$}
\begin{mathpar}
  \inferrule
      {p \to^a p'}
      {C[T[p]]\; {}^s\!\!\to^a C[T[p']]}

  \inferrule
      {~}
      {C[SA(AS(e))] \;{}^s\!\!\to^a C[e]}

  \inferrule
      {~}
      {C[AS(SA(M))] \;{}^s\!\!\to^a C[M]}
\end{mathpar}

\fbox{$H;\; p \to^p H;\; p$}
\begin{mathpar}
  \inferrule*[right=\text{Step-S1}]
      {H\; e \to H';\; e'}
      {H;\; e \to^p H';\; e'}

  \inferrule*[right=\text{Step-S2}]
      {H\; e \to H';\; e'}
      {H;\; AS(e) \to^p H';\; AS(e')}

  \inferrule*[right=\text{Step-T1}]
      {H\; M \to H';\; M'}
      {H;\; M \to^p H';\; M'}

  \inferrule*[right=\text{Step-T2}]
      {H\; M \to H';\; M'}
      {H;\; SA(M) \to^p H';\; SA(M')}

  \inferrule*[right=\text{Step-Across}]
      {M \; {}^s\!\!\to^a M'}
      {H;\; M \to^p H;\; M'}
\end{mathpar}


\fbox{$e \Downarrow_{AOT} M$}
\begin{mathpar}
  \inferrule
             {AS(e) \; {}^s\!\!\to^a\!\!*\; M
               \\
               M \; {}^s\!\!\not\to^a M'}
      {e \Downarrow_{AOT} M}
\end{mathpar}

\newtheorem{proposition}{Proposition}
\newtheorem{corollary}{Corollary}
\newtheorem{theorem}{Theorem}

\begin{proposition}[Confluence]
  ~\\
  If $H; p \to^{p*}  H_1; p_1$  and
  $H; p \to^{p*}  H_2; p_2$ then \\
  $H_1; p_1  \to^{p*} H'; p'$ and
  $H_2; p_2  \to^{p*} H'; p'$.
\end{proposition}

\begin{corollary}[Whole-Program Correctness]
  ~\\
  If $\cdot; e \to^{p*}  H_1; v$  and
  $e \Downarrow_{AOT} M$ then \\
  $\cdot; M  \to^{p*} H_2; v$
\end{corollary}

\begin{proposition}[Type Preservation]
  ~\\
  If $\Gamma \vdash e : A$ and $e \Downarrow_{AOT} M$ then $\Gamma' \vdash M : B$ (ish)
\end{proposition}

\begin{proposition}[Subject Reduction]
~\\
  If $\Gamma \vdash e : A$ and $H; e \to^{p} H'; e'$ then $\Gamma \vdash e' : A$
\end{proposition}

\begin{theorem}[Subject Reduction Implies Type Safety]
~\\
  If ($\Gamma \vdash e : A$ and $H; e \to^{p} H'; e'$ implies $\Gamma \vdash e' : A$) then\\
  ($\Gamma \vdash e : A$ and $e \Downarrow_{AOT} M$ implies $\Gamma' \vdash M : B$)
\end{theorem}

\newtheorem{definition}{Definition}
\newtheorem{lemma}{Lemma}

\begin{definition}[Contextual Equivalence]
  ~\\
  \begin{displaymath}
    \begin{array}{rclcl}
      H_1; p_1 & \approx_{SA} & H_2; p_2 &\defeq& \forall C. H_1; C[p_1] \Downarrow^p \iff H_2; C[p_2] \Downarrow^p\\
      H_1; e_1 & \approx_{S} & H_2; e_2 &\defeq& \forall C_S. H_1; C_S[e_1] \Downarrow^s \iff H_2; C_S[e_2] \Downarrow^s\\
      H_1; M_1 & \approx_{A} & H_2; M_2 &\defeq& \forall C_A. H_1; C_A[M_1] \Downarrow^a \iff H_2; C_A[M_2] \Downarrow^a
      \end{array}
  \end{displaymath}
\end{definition}

\begin{proposition}[Full Abstraction]
  ~\\
  Suppose $e_1 \Downarrow_{AOT} M_1$ and $e_2 \Downarrow_{AOT} M_2$.\\
  $H_1; e_1 \approx_S H_2; e_2$ if and only if $H_1; M_1 \approx_A H_2; M_2$.
\end{proposition}

\begin{lemma}[Full Abstraction (hard part)]
  ~\\
  Suppose $e_1 \Downarrow_{AOT} M_1$ and $e_2 \Downarrow_{AOT} M_2$.\\
  $H_1; e_1 \approx_S H_2; e_2$ if and only if $H_1; M_1 \approx_{SA} H_2; M_2$.
\end{lemma}

\begin{lemma}[Full Abstraction (easy part)]
  ~\\
  Suppose $e_1 \Downarrow_{AOT} M_1$ and $e_2 \Downarrow_{AOT} M_2$.\\
  $H_1; e_1 \approx_{SA} H_2; e_2$ if and only if $H_1; M_1 \approx_{A} H_2; M_2$.
\end{lemma}



\end{document}
